UTP/ITree_Hoare.thy
@@ -9,22 +9,18 @@ named_theorems hoare_safe
 definition hoare_triple :: "('s \<Rightarrow> bool) \<Rightarrow> ('e, 's) htree \<Rightarrow> ('s \<Rightarrow> bool) \<Rightarrow> bool" where
 "hoare_triple P S Q = (itree_rel S \<subseteq> spec \<top>\<^sub>S P Q)"
 
-abbreviation hoare_preserves :: "('e, 's) htree \<Rightarrow> ('s \<Rightarrow> bool) \<Rightarrow> bool" where
-"hoare_preserves S P \<equiv> hoare_triple P S P"
-
-abbreviation hoare_establishes :: "'s subst \<Rightarrow> ('s \<Rightarrow> bool) \<Rightarrow> bool" where
-"hoare_establishes \<sigma> P \<equiv> hoare_triple (True)\<^sub>e (\<langle>\<sigma>\<rangle>\<^sub>a :: (unit, 's) htree) P"
-
 syntax 
-  "_hoare" :: "logic \<Rightarrow> logic \<Rightarrow> logic \<Rightarrow> logic" ("\<^bold>{_\<^bold>}/ _/ \<^bold>{_\<^bold>}")
-  "_hoare" :: "logic \<Rightarrow> logic \<Rightarrow> logic \<Rightarrow> logic" ("H{_}/ _/ {_}")
-  "_preserves" :: "logic \<Rightarrow> logic \<Rightarrow> logic" (infix "preserves" 55)
-  "_establishes" :: "logic \<Rightarrow> logic \<Rightarrow> logic" (infix "establishes" 55)
+  "_hoare"           :: "logic \<Rightarrow> logic \<Rightarrow> logic \<Rightarrow> logic" ("\<^bold>{_\<^bold>}/ _/ \<^bold>{_\<^bold>}")
+  "_hoare"           :: "logic \<Rightarrow> logic \<Rightarrow> logic \<Rightarrow> logic" ("H{_}/ _/ {_}")
+  "_preserves"       :: "logic \<Rightarrow> logic \<Rightarrow> logic" (infix "preserves" 55)
+  "_preserves_under" :: "logic \<Rightarrow> logic \<Rightarrow> logic \<Rightarrow> logic" ("_ preserves _ under _" [55, 0, 55] 55)
+  "_establishes"     :: "logic \<Rightarrow> logic \<Rightarrow> logic" (infix "establishes" 55)
 
 translations
   "_hoare P S Q" == "CONST hoare_triple (P)\<^sub>e S (Q)\<^sub>e"
-  "_preserves S P" == "CONST hoare_preserves S (P)\<^sub>e"
-  "_establishes S P" == "CONST hoare_establishes S (P)\<^sub>e"
+  "_preserves S P" => "H{P} S {P}"
+  "_preserves_under S P Q" => "H{P \<and> Q} S {P}"
+  "_establishes \<sigma> P" => "H{CONST True} \<langle>\<sigma>\<rangle>\<^sub>a {P}"
 
 lemma hoare_alt_def: "\<^bold>{P\<^bold>} S \<^bold>{Q\<^bold>} \<longleftrightarrow> (\<forall> s s' es. P s \<and> S s \<midarrow>es\<leadsto> \<checkmark> s' \<longrightarrow> Q s')"
   by (auto simp add: hoare_triple_def spec_def itree_rel_def retvals_def subset_iff)
